SlowTest/DiffLogic-Test/seq2_Dafny.dfy
@@ -1,48 +1,51 @@
 // dafny/Test/dafny4/git-issue96.dfy
 
+function method add(x: int, y: int) : int { x + y }
 
 lemma addition_bound_instance ()
-    ensures forall i, j {:trigger i + j} :: 0 <= i && 0 <= j ==> 0 <= i + j
-    ensures forall i, j {:trigger i + j} :: i < 5 && j < 5 ==> i + j < 10
+    ensures forall i, j {:trigger add(i, j)} :: 0 <= i && 0 <= j ==> 0 <= add(i, j)
+    ensures forall i, j {:trigger add(i, j)} :: i < 5 && j < 5 ==> add(i, j) < 10
 
-lemma addition_bound (l: int, h: int)
-    ensures forall i, j {:trigger i + j} :: l <= i && l <= j ==> l + l <= i + j
-    ensures forall i, j {:trigger i + j} :: i < h && j < h ==> i + j < h + h
+lemma addition_bound (i: int, j: int, l: int, h: int)
+    ensures l <= i && l <= j ==> l + l <= add(i, j)
+    ensures i < h && j < h ==> add(i, j) < h + h
 
-predicate P(s:seq<int>)
+// predicate P(s:seq<int>)
+//     requires 10 < |s|
+// {
+//     addition_bound_instance ();
+//     (forall i:int {:trigger s[i]} :: forall j:int {:trigger s[j]} ::
+//         0 <= i < j < 5 ==> s[add(i, j)] == s[i] == s[j])
+// }
+
+// predicate P0(s:seq<int>)
+//     requires 10 < |s|
+// {
+//     addition_bound_instance ();
+//     (forall i:int :: forall j:int ::
+//         0 <= i < j < 5 ==> s[add(i, j)] == s[i] == s[j])
+// }
+
+// predicate P1(s:seq<int>)
+method P1(s:seq<int>) returns (b: bool)
     requires 10 < |s|
 {
-    addition_bound_instance ();
-    assume (forall i, j {:trigger i + j} :: i + j < 10 ==> i + j < |s|);
-    (forall i:int {:trigger s[i]} :: forall j:int {:trigger s[j]} ::
-        0 <= i < j < 5 ==> s[i + j] == s[i] == s[j])
+    forall i: int, j: int | 0 <= i < j < 5
+        ensures 0 <= add(i, j)
+        ensures add(i, j) < 10
+        {
+            // addition_bound_instance ();
+            addition_bound(i, j, 0, 5); // doesn't work
+        }
+
+    // (forall i:int, j: int {:trigger s[i], s[j]} :: 0 <= i < j < 5 ==> s[add(i, j)] == s[i]+s[j])
+    b := (forall i:int, j: int {:trigger s[i], s[j]} :: 0 <= i < j < 5 ==> s[add(i, j)] == s[i]+s[j]);
 }
 
-predicate P0(s:seq<int>)
-    requires 10 < |s|
-{
-    addition_bound_instance ();
-    assume (forall i, j {:trigger i + j} :: i + j < 10 ==> i + j < |s|);
-    (forall i:int :: forall j:int ::
-        0 <= i < j < 5 ==> s[i + j] == s[i] == s[j]) // not work?
-}
-
-predicate P1(s:seq<int>)
-    requires 10 < |s|
-{
-    addition_bound_instance ();
-    // addition_bound (0, 5); // not work
-    assume (forall i, j {:trigger i + j} :: i + j < 10 ==> i + j < |s|);
-
-    (forall i:int, j: int {:trigger s[i], s[j]} ::
-        0 <= i < j < 5 ==> s[i + j] == s[i]+s[j])
-}
-
-predicate P2(s:seq<int>)
-    requires 10 < |s|
-{
-    addition_bound_instance ();
-    assume (forall i, j {:trigger i + j} :: i + j < 10 ==> i + j < |s|);
-    (forall i:int, j: int ::
-        0 <= i < j < 5 ==> s[i + j] == s[i]+s[j])
-}
+// predicate P2(s:seq<int>)
+//     requires 10 < |s|
+// {
+//     addition_bound_instance ();
+//     (forall i:int, j: int ::
+//         0 <= i < j < 5 ==> s[add(i, j)] == s[i]+s[j])
+// }
