SlowTest/DiffLogic-Test/seq2-Boogie2Boogie.bpl
@@ -1,0 +1,35 @@
+// Boogie program verifier version 2.4.1.10503, Copyright (c) 2003-2014, Microsoft.
+// Command Line Options: seq2_Boogie.bpl /trace /proverOpt:O:smt.arith.solver=3 /proverOpt:LOGIC=DLA /print:seq2-Boogie2Boogie.bpl /proverLog:seq2-Boogie2z3.smt2
+
+function add(x: int, y: int) : int;
+
+axiom (forall x: int, y: int :: { add(x, y): int } add(x, y): int == x + y);
+
+procedure bound(i: int, j: int, l: int, h: int);
+  ensures i >= l && j >= l ==> l + l <= add(i, j);
+  ensures i < h && j < h ==> add(i, j) < h + h;
+
+
+
+procedure bound2(l: int, h: int);
+  ensures (forall i: int, j: int :: i >= l && j >= l ==> l + l < add(i, j));
+  ensures (forall i: int, j: int :: i < h && j < h ==> add(i, j) < h + h);
+
+
+
+procedure P(i: int, j: int, l: int);
+  requires l > 10;
+
+
+
+implementation P(i: int, j: int, l: int)
+{
+    call bound2(0, 5);
+    if (0 <= i && i < j && j < 5)
+    {
+        assert 0 <= add(i, j);
+        assert add(i, j) < l;
+    }
+}
+
+
