SlowTest/DiffLogic-Test/seq2-Boogie2z3.smt2
@@ -1,0 +1,57 @@
+(set-option :print-success false)
+(set-info :smt-lib-version 2.0)
+(set-option :smt.arith.solver 3)
+(set-option :AUTO_CONFIG false)
+(set-option :pp.bv_literals false)
+(set-option :MODEL.V2 true)
+(set-option :smt.PHASE_SELECTION 0)
+(set-option :smt.RESTART_STRATEGY 0)
+(set-option :smt.RESTART_FACTOR |1.5|)
+(set-option :smt.ARITH.RANDOM_INITIAL_VALUE true)
+(set-option :smt.CASE_SPLIT 3)
+(set-option :smt.DELAY_UNITS true)
+(set-option :NNF.SK_HACK true)
+(set-option :smt.MBQI false)
+(set-option :smt.QI.EAGER_THRESHOLD 100)
+(set-option :TYPE_CHECK true)
+(set-option :smt.BV.REFLECT true)
+(set-option :model.compact false)
+(set-logic DLA)
+; done setting options
+
+
+(declare-fun tickleBool (Bool) Bool)
+(assert (and (tickleBool true) (tickleBool false)))
+(declare-fun add (Int Int) Int)
+(assert (forall ((x Int) (y Int) ) (! (= (add x y) (+ x y))
+ :qid |seq2Boog.1:14|
+ :skolemid |0|
+ :pattern ( (add x y))
+)))
+(declare-fun %lbl%+0 () Bool)
+(declare-fun %lbl%+1 () Bool)
+(declare-fun i () Int)
+(declare-fun j () Int)
+(declare-fun %lbl%@2 () Bool)
+(declare-fun %lbl%@3 () Bool)
+(declare-fun l () Int)
+(declare-fun %lbl%+4 () Bool)
+(declare-fun %lbl%+5 () Bool)
+(push 1)
+(set-info :boogie-vc-id P)
+(assert (not
+(let ((anon2_Else_correct  (=> (! (and %lbl%+0 true) :lblpos +0) true)))
+(let ((anon2_Then_correct  (=> (! (and %lbl%+1 true) :lblpos +1) (=> (and (and (<= 0 i) (< i j)) (< j 5)) (and (! (or %lbl%@2 (<= 0 (add i j))) :lblneg @2) (=> (<= 0 (add i j)) (! (or %lbl%@3 (< (add i j) l)) :lblneg @3)))))))
+(let ((anon0_correct  (=> (! (and %lbl%+4 true) :lblpos +4) (=> (and (forall ((i@@0 Int) (j@@0 Int) ) (!  (=> (and (>= i@@0 0) (>= j@@0 0)) (< (+ 0 0) (add i@@0 j@@0)))
+ :qid |seq2Boog.9:21|
+ :skolemid |1|
+)) (forall ((i@@1 Int) (j@@1 Int) ) (!  (=> (and (< i@@1 5) (< j@@1 5)) (< (add i@@1 j@@1) (+ 5 5)))
+ :qid |seq2Boog.10:21|
+ :skolemid |2|
+))) (and anon2_Then_correct anon2_Else_correct)))))
+(let ((PreconditionGeneratedEntry_correct  (=> (! (and %lbl%+5 true) :lblpos +5) (=> (> l 10) anon0_correct))))
+PreconditionGeneratedEntry_correct))))
+))
+(check-sat)
+(pop 1)
+; Valid
